Classes/Monad/MonadJoin.v
@@ -1,7 +1,7 @@
 Require Export Base.
 Require Import Classes.Monad Classes.Joinable Classes.Galois.
 
-Class MonadJoin M {MM : Monad M} : Type := {
+Class MonadJoin M `{MM : Monad M} : Type := {
   mjoin : ∀ {A} {JA : Joinable A A} {JI : JoinableIdem JA}, M A → M A → M A;
   mjoin_return : ∀ {A} {JA : Joinable A A} {JI : JoinableIdem JA} (x y : A),
     mjoin (returnM x) (returnM y) = returnM (x ⊔ y);
@@ -9,8 +9,8 @@ Class MonadJoin M {MM : Monad M} : Type := {
 Hint Rewrite @mjoin_return : monads.
 Infix "<⊔>" := mjoin (at level 40).
 
-Class MonadJoinSound (M M' : Type → Type) {MM : Monad M} {MJ : MonadJoin M}
-  {MM' : Monad M'} {GM : ∀ A A', Galois A A' → Galois (M A) (M' A')} : Type :=
+Class MonadJoinSound (M M' : Type → Type) `{MM : Monad M} {MJ : MonadJoin M}
+  `{MM' : Monad M'} {GM : ∀ A A', Galois A A' → Galois (M A) (M' A')} : Type :=
 {
   mjoin_sound_left : ∀ {A A'} {JA : Joinable A A} {JAI : JoinableIdem JA} 
     {GA : Galois A A'} {JS : JoinableSound JA} (m1 m2 : M A) (m' : M' A'),
