Instances/Store.v
@@ -18,13 +18,13 @@ Proof.
 Qed.
 Hint Resolve get_store_state_sound : soundness.
 
-Instance store_stateT {S} {M} {MM : Monad M} : MonadState S (StateT S M) := {
+Instance store_stateT {S} {M} `{MM : Monad M} : MonadState S (StateT S M) := {
   get := λ st, returnM (st, st);
   put := λ st, λ _, returnM (tt, st);
 }.
 
 Instance get_store_stateT_sound {ST ST' : Type} {GS : Galois ST ST'} 
-  {M M' : Type → Type} {MM : Monad M} {MM' : Monad M'}
+  {M M' : Type → Type} `{MM : Monad M} `{MM' : Monad M'}
   {GM : ∀ A A', Galois A A' → Galois (M A) (M' A')} :
   return_sound M M' →
   get_state_sound (StateT ST M) (StateT ST' M').
@@ -34,7 +34,7 @@ Qed.
 Hint Resolve get_store_stateT_sound : soundness.
 
 Instance put_store_stateT_sound {ST ST' : Type} {GS : Galois ST ST'}
-  {M M' : Type → Type} {MM : Monad M} {MM' : Monad M'}
+  {M M' : Type → Type} `{MM : Monad M} `{MM' : Monad M'}
   {GM : ∀ A A', Galois A A' → Galois (M A) (M' A')} :
   return_sound M M' →
   put_state_sound (StateT ST M) (StateT ST' M').
@@ -44,14 +44,14 @@ Proof.
 Qed.
 Hint Resolve put_store_stateT_sound : soundness.
 
-Instance store_optionT {ST} {M} {MM : Monad M} {MS : MonadState ST M} :
+Instance store_optionT {ST} {M} `{MM : Monad M} {MS : MonadState ST M} :
   MonadState ST (optionT M) := {
   get := get >>= λ a, returnM (Some a);
   put := λ st, put st ;; returnM (Some tt);
 }.
 
 Instance get_store_optionT_sound {ST ST' : Type} {GST : Galois ST ST'}
-  {M M' : Type → Type} {MM : Monad M} {MM' : Monad M'}
+  {M M' : Type → Type} `{MM : Monad M} `{MM' : Monad M'}
   {GM : ∀ A A', Galois A A' → Galois (M A) (M' A')}
   {MS : MonadState ST M} {MS' : MonadState ST' M'} :
   bind_sound M M' →
